11FlatMemory/FlatMemory.thy
@@ -10,6 +10,8 @@ fun get_closure :: "nat heap \<Rightarrow> nat \<Rightarrow> ceclosure" where
       0 \<Rightarrow> CEConst (hlookup h (Suc p))
     | Suc x \<Rightarrow> CELam (hlookup h (Suc p)) (hlookup h (Suc (Suc p))))"
 
+declare get_closure.simps [simp del]
+
 fun flat_lookup :: "ptr heap \<Rightarrow> ptr \<Rightarrow> nat \<rightharpoonup> ptr" where
   "flat_lookup h 0 x = None"
 | "flat_lookup h (Suc 0) x = None"
@@ -24,13 +26,12 @@ inductive evalf :: "byte_code list \<Rightarrow> flat_state \<Rightarrow> flat_s
 | evf_pushlam [simp]: "cd ! pc = BPushLam pc' \<Longrightarrow> halloc_list h [1, p, pc'] = (h', v) \<Longrightarrow> 
     cd \<tturnstile> FS h env vs (Suc pc # p # sfs) \<leadsto>\<^sub>f FS h' env (v # vs) (pc # p # sfs)"
 | evf_apply [simp]: "cd ! pc = BApply \<Longrightarrow> get_closure h v2 = CELam p' pc' \<Longrightarrow>
-    halloc env v1 = (env1, p1) \<Longrightarrow> halloc env1 p' = (env2, p2) \<Longrightarrow> 
-      cd \<tturnstile> FS h env (v1 # v2 # vs) (Suc pc # p # sfs) \<leadsto>\<^sub>f 
-        FS h env2 vs (pc' # Suc p2 # pc # p # sfs)"
+    halloc_list env [v1, p'] = (env', p2) \<Longrightarrow> 
+      cd \<tturnstile> FS h env (v1 # v2 # vs) (Suc pc # p # sfs) \<leadsto>\<^sub>f FS h env' vs (pc' # Suc p2 # pc # p # sfs)"
 | evf_return [simp]: "cd ! pc = BReturn \<Longrightarrow> cd \<tturnstile> FS h env vs (Suc pc # p # sfs) \<leadsto>\<^sub>f FS h env vs sfs"
 | evf_jump [simp]: "cd ! pc = BJump \<Longrightarrow> get_closure h v2 = CELam p' pc' \<Longrightarrow>
-    halloc env v1 = (env1, p1) \<Longrightarrow> halloc env1 p' = (env2, p2) \<Longrightarrow> 
-      cd \<tturnstile> FS h env (v1 # v2 # vs) (Suc pc # p # sfs) \<leadsto>\<^sub>f FS h env2 vs (pc' # Suc p2 # sfs)"
+    halloc_list env [v1, p'] = (env', p2) \<Longrightarrow> 
+      cd \<tturnstile> FS h env (v1 # v2 # vs) (Suc pc # p # sfs) \<leadsto>\<^sub>f FS h env' vs (pc' # Suc p2 # sfs)"
 
 theorem determinismf: "cd \<tturnstile> \<Sigma> \<leadsto>\<^sub>f \<Sigma>' \<Longrightarrow> cd \<tturnstile> \<Sigma> \<leadsto>\<^sub>f \<Sigma>'' \<Longrightarrow> \<Sigma>' = \<Sigma>''"
 proof (induction \<Sigma> \<Sigma>' rule: evalf.induct)
@@ -46,16 +47,16 @@ next
   from evf_pushlam(3, 1, 2) show ?case 
     by (induction cd "FS h env vs (Suc pc # p # sfs)" \<Sigma>'' rule: evalf.induct) simp_all 
 next
-  case (evf_apply cd pc h v2 p' pc' env v1 env1 p1 env2 p2 vs p sfs)
-  from evf_apply(5, 1, 2, 3, 4) show ?case 
+  case (evf_apply cd pc h v2 p' pc' env v1 env' p2 vs p sfs)
+  from evf_apply(4, 1, 2, 3) show ?case 
     by (induction cd "FS h env (v1 # v2 # vs) (Suc pc # p # sfs)" \<Sigma>'' rule: evalf.induct) simp_all 
 next
   case (evf_return cd pc h env vs p sfs)
   from evf_return(2, 1) show ?case 
     by (induction cd "FS h env vs (Suc pc # p # sfs)" \<Sigma>'' rule: evalf.induct) simp_all 
 next
-  case (evf_jump cd pc h v2 p' pc' env v1 env1 p1 env2 p2 vs p sfs)
-  from evf_jump(5, 1, 2, 3, 4) show ?case 
+  case (evf_jump cd pc h v2 p' pc' env v1 env' p2 vs p sfs)
+  from evf_jump(4, 1, 2, 3) show ?case 
     by (induction cd "FS h env (v1 # v2 # vs) (Suc pc # p # sfs)" \<Sigma>'' rule: evalf.induct) simp_all 
 qed
 
